---
title: "ç·šå½¢ã‚·ã‚¹ãƒ†ãƒ ã®å‹‰å¼·ãƒãƒ¼ãƒˆ"
emoji: "ğŸ–‹"
type: "tech" # tech: æŠ€è¡“è¨˜äº‹ / idea: ã‚¢ã‚¤ãƒ‡ã‚¢
topics: ["math"]
published: false
---
# 2æ¬¡å…ƒç·šå½¢ã‚·ã‚¹ãƒ†ãƒ 

2æ¬¡å…ƒç·šå½¢ã‚·ã‚¹ãƒ†ãƒ 

$$
\begin{aligned}
\dot{\vec{x}} = \mathbf{A}\vec{x}\\
\end{aligned}
$$

2æ¬¡å…ƒè¡Œåˆ—

$$
\begin{aligned}
\mathbf{A} = \begin{bmatrix}
a & b\\
c & d
\end{bmatrix}
\end{aligned}
$$

å›ºæœ‰å€¤: $\lambda_1, \lambda_2$
å›ºæœ‰ãƒ™ã‚¯ãƒˆãƒ«: $\vec{v}_1, \vec{v}_2$

ä¸€èˆ¬è§£

$$
\begin{aligned}
\vec{x} = c_1 e^{\lambda_1 t} \vec{v}_1 + c_2 e^{\lambda_2 t} \vec{v}_2\\
\end{aligned}
$$

---

## ä¾‹

### ä¾‹1

$$
\begin{aligned}
\frac{ dx }{ dt } &= ax + by\\
\frac{ dy }{ dt } &= -bx - ay\\
\end{aligned}
$$

ãŸã ã—ï¼Œ$a, b > 0$ï¼

1. è¡Œåˆ—å½¢å¼ã§æ›¸ãï¼

$$
\begin{aligned}
\dot{\vec{x}} = \begin{bmatrix}
\frac{ d x }{ d t }\\
\frac{ d y }{ d t }
\end{bmatrix} &= 
\mathbf{A}\vec{x}\\
&= \begin{bmatrix}
a & b\\
-b & -a
\end{bmatrix}
\begin{bmatrix}
x \\ y
\end{bmatrix}
\end{aligned}
$$

2. $\mathbf{A}$ã®å›ºæœ‰å€¤$\lambda_1, \lambda_2$ã‚’æ±‚ã‚ã‚‹ï¼

$$
\begin{aligned}
\det(\mathbf{A} - \lambda \mathbf{I}) &= 0\\
\begin{vmatrix}
a - \lambda & b\\
-b & -a - \lambda
\end{vmatrix} &= 0\\
(a - \lambda)(-a - \lambda) - b(-b) &= 0\\
(\lambda - a)(\lambda + a) + b^2 &= 0\\
\lambda^2 - a^2 + b^2 &= 0\\
\lambda^2 &= a^2 - b^2\\
\lambda &= \pm \sqrt{a^2 - b^2}\\
\lambda_1, \lambda_2 &= + \sqrt{a^2 - b^2}, -\sqrt{a^2 - b^2}\\
\end{aligned}
$$

3. å›ºæœ‰ãƒ™ã‚¯ãƒˆãƒ«$\vec{v}_1, \vec{v}_2$ã‚’æ±‚ã‚ã‚‹ï¼

$$
\begin{aligned}
(\mathbf{A} - \lambda \mathbf{I})\vec{v} &= \mathbf{0}\\
\end{aligned}
$$

$\lambda_1 = + \sqrt{a^2 - b^2}$ã®å ´åˆï¼Œ

$$
\begin{aligned}
\begin{bmatrix}
a - \sqrt{a^2 - b^2} & b\\
-b & -a - \sqrt{a^2 - b^2}
\end{bmatrix}
\begin{bmatrix}
v_x \\ v_y
\end{bmatrix} &= 
\begin{bmatrix}
0 \\ 0
\end{bmatrix}\\
\end{aligned}
$$

$$
\begin{aligned}
\vec{v}_1 = \begin{bmatrix}
v_x \\ v_y
\end{bmatrix} &= 
\begin{bmatrix}
{ a + \sqrt{a^2 - b^2} }\\
-b\\
\end{bmatrix}\\
&= 
\begin{bmatrix}
{ \frac{ a }{ b } + \sqrt{\left(\frac{ a }{ b }\right)^2 - 1} }\\
-1\\
\end{bmatrix}\\
\end{aligned}
$$

$\lambda_2 = - \sqrt{a^2 - b^2}$ã®å ´åˆï¼Œ

$$
\begin{aligned}
\begin{bmatrix}
a + \sqrt{a^2 - b^2} & b\\
-b & -a + \sqrt{a^2 - b^2}
\end{bmatrix}
\begin{bmatrix}
v_x \\ v_y
\end{bmatrix} &= 
\begin{bmatrix}
0 \\ 0
\end{bmatrix}\\
\end{aligned}
$$

$$
\begin{aligned}
\vec{v}_2 = \begin{bmatrix}
v_x \\ v_y
\end{bmatrix} &= 
\begin{bmatrix}
{ \frac{ a }{ b } - \sqrt{\left(\frac{ a }{ b }\right)^2 - 1} }\\
-1\\
\end{bmatrix}
\end{aligned}
$$

---

### ä¾‹2

$$
\begin{aligned}
\mathbf{A} &= 
\begin{bmatrix}
a & b\\
b & a
\end{bmatrix}\\
\end{aligned}
$$

å›ºæœ‰å€¤ã‚’æ±‚ã‚ã‚‹ï¼

$$
\begin{aligned}
\begin{vmatrix}
a - \lambda & b\\
b & a - \lambda
\end{vmatrix} &= 0\\
(a - \lambda)^2 - b^2 &= 0\\
a - \lambda &= \pm b\\
\lambda &= a \pm b\\
\lambda_1, \lambda_2 &= a + b, a - b\\
\end{aligned}
$$

å›ºæœ‰ãƒ™ã‚¯ãƒˆãƒ«ã‚’æ±‚ã‚ã‚‹ï¼

$$
\begin{aligned}
\begin{bmatrix}
a - (a + b) & b\\
b & a - (a + b)
\end{bmatrix}\vec{v}_1 &= 0\\
\begin{bmatrix}
-b & b\\
b & -b
\end{bmatrix}\vec{v}_1 &= 0\\
\vec{v}_1 &= 
\begin{bmatrix}
1 \\ 1
\end{bmatrix}
\end{aligned}
$$

$$
\begin{aligned}
\begin{bmatrix}
a - (a - b) & b\\
b & a - (a - b)
\end{bmatrix}
\vec{v}_2 &= \vec{0}\\
\begin{bmatrix}
b & b\\
b & b
\end{bmatrix}
\vec{v}_2 &= \vec{0}\\
\vec{v}_2 &= \begin{bmatrix}
1 \\ -1
\end{bmatrix}\\
\end{aligned}
$$

ã‚°ãƒ©ãƒ•ã«æãéš›ã¯ï¼Œå›ºæœ‰ãƒ™ã‚¯ãƒˆãƒ«æ–¹å‘ã¯å›ºæœ‰å€¤å€ã«ãªã‚‹ã“ã¨ã‚’æ„è­˜ã™ã‚‹ï¼